

Question 3: Baby Convolutional Neural Network Solution

(a) Compute gradients $\frac{\partial h}{\partial \theta_j}$ and $\frac{\partial h}{\partial w_j}$ [6 marks]

Given:

$$u_1 = \theta_1 x_1 + \theta_2 x_2 + \theta_3 x_4 + \theta_4 x_5 \quad (1)$$

$$u_2 = \theta_1 x_2 + \theta_2 x_3 + \theta_3 x_5 + \theta_4 x_6 \quad (2)$$

$$u_3 = \theta_1 x_4 + \theta_2 x_5 + \theta_3 x_7 + \theta_4 x_8 \quad (3)$$

$$u_4 = \theta_1 x_5 + \theta_2 x_6 + \theta_3 x_8 + \theta_4 x_9 \quad (4)$$

$$h = \frac{1}{1 + e^{-(w_1 u_1 + w_2 u_2 + w_3 u_3 + w_4 u_4)}} \quad (5)$$

Let $z = w_1 u_1 + w_2 u_2 + w_3 u_3 + w_4 u_4$, so $h = \frac{1}{1 + e^{-z}} = \sigma(z)$.

Using the chain rule:

$$\frac{\partial h}{\partial \theta_j} = \frac{\partial h}{\partial z} \cdot \frac{\partial z}{\partial \theta_j} \quad (6)$$

$$\frac{\partial h}{\partial w_j} = \frac{\partial h}{\partial z} \cdot \frac{\partial z}{\partial w_j} \quad (7)$$

First, compute $\frac{\partial h}{\partial z}$:

$$\frac{\partial h}{\partial z} = \frac{\partial}{\partial z} \left(\frac{1}{1 + e^{-z}} \right) = \frac{e^{-z}}{(1 + e^{-z})^2} = h(1 - h) \quad (8)$$

Next, compute $\frac{\partial z}{\partial \theta_j}$:

$$\frac{\partial z}{\partial \theta_1} = w_1 x_1 + w_2 x_2 + w_3 x_4 + w_4 x_5 \quad (9)$$

$$\frac{\partial z}{\partial \theta_2} = w_1 x_2 + w_2 x_3 + w_3 x_5 + w_4 x_6 \quad (10)$$

$$\frac{\partial z}{\partial \theta_3} = w_1 x_4 + w_2 x_5 + w_3 x_7 + w_4 x_8 \quad (11)$$

$$\frac{\partial z}{\partial \theta_4} = w_1 x_5 + w_2 x_6 + w_3 x_8 + w_4 x_9 \quad (12)$$

And $\frac{\partial z}{\partial w_j}$:

$$\frac{\partial z}{\partial w_1} = u_1, \quad \frac{\partial z}{\partial w_2} = u_2, \quad \frac{\partial z}{\partial w_3} = u_3, \quad \frac{\partial z}{\partial w_4} = u_4 \quad (13)$$

Therefore:

$$\frac{\partial h}{\partial \theta_1} = h(1-h)(w_1x_1 + w_2x_2 + w_3x_4 + w_4x_5) \quad (14)$$

$$\frac{\partial h}{\partial \theta_2} = h(1-h)(w_1x_2 + w_2x_3 + w_3x_5 + w_4x_6) \quad (15)$$

$$\frac{\partial h}{\partial \theta_3} = h(1-h)(w_1x_4 + w_2x_5 + w_3x_7 + w_4x_8) \quad (16)$$

$$\frac{\partial h}{\partial \theta_4} = h(1-h)(w_1x_5 + w_2x_6 + w_3x_8 + w_4x_9) \quad (17)$$

$$\frac{\partial h}{\partial w_1} = h(1-h)u_1, \quad \frac{\partial h}{\partial w_2} = h(1-h)u_2, \quad \frac{\partial h}{\partial w_3} = h(1-h)u_3, \quad \frac{\partial h}{\partial w_4} = h(1-h)u_4 \quad (18)$$

(b) Derive the negative log-likelihood function [3 marks]

For binary classification with training dataset $\{(x_i, y_i)\}_{i=1}^N$ where $x_i \in \mathbb{R}^9$ and $y_i \in \{0, 1\}$:

The likelihood for each data point is:

$$P(y_i|x_i) = h_i^{y_i}(1-h_i)^{1-y_i}$$

where $h_i = h(x_i, \theta, w)$.

The total likelihood is:

$$L(\theta, w) = \prod_{i=1}^N P(y_i|x_i) = \prod_{i=1}^N h_i^{y_i}(1-h_i)^{1-y_i}$$

The log-likelihood is:

$$\ell(\theta, w) = \sum_{i=1}^N [y_i \log h_i + (1-y_i) \log(1-h_i)]$$

Therefore, the negative log-likelihood function to minimize is:

$$\boxed{\text{NLL}(\theta, w) = - \sum_{i=1}^N [y_i \log h_i + (1-y_i) \log(1-h_i)]}$$

This is the binary cross-entropy loss function.

(c) SGD Algorithm with Mini-batch [8 marks]

Mini-batch SGD proceeds by first sampling a batch of datapoints $\mathcal{B} = \{j_1, j_2, \dots, j_{32}\}$, and then perform the updates

$$\theta^{t+1} = \theta^t - \alpha \cdot h_\theta(\theta^t, w^t; \mathcal{B}) \quad (19)$$

$$w^{t+1} = w^t - \alpha \cdot h_w(\theta^t, w^t; \mathcal{B}) \quad (20)$$

where $h_\theta(\theta^t, w^t; \mathcal{B})$ and $h_w(\theta^t, w^t; \mathcal{B})$ are computed as the average gradients over the batch \mathcal{B} :

$$h_\theta(\theta^t, w^t; \mathcal{B}) = \frac{1}{|\mathcal{B}|} \sum_{j \in \mathcal{B}} h_\theta(\theta^t, w^t; j) \quad (21)$$

$$h_w(\theta^t, w^t; \mathcal{B}) = \frac{1}{|\mathcal{B}|} \sum_{j \in \mathcal{B}} h_w(\theta^t, w^t; j) \quad (22)$$

where for each individual sample j in the batch:

- If $y_j = 1$, by the chain rule,

$$h_\theta(\theta^t, w^t; j) = \frac{\partial(-\ln h_j)}{\partial \theta} = -\frac{1}{h_j} \cdot \frac{\partial h_j}{\partial \theta} \quad (23)$$

$$= -\frac{1}{h_j} \cdot h_j(1 - h_j) \cdot \frac{\partial z_j}{\partial \theta} \quad (24)$$

$$= -(1 - h_j) \cdot \frac{\partial z_j}{\partial \theta} \quad (25)$$

$$h_w(\theta^t, w^t; j) = \frac{\partial(-\ln h_j)}{\partial w} = -\frac{1}{h_j} \cdot \frac{\partial h_j}{\partial w} \quad (26)$$

$$= -\frac{1}{h_j} \cdot h_j(1 - h_j) \cdot \frac{\partial z_j}{\partial w} \quad (27)$$

$$= -(1 - h_j) \cdot u_j \quad (28)$$

- If $y_j = 0$, by the chain rule,

$$h_\theta(\theta^t, w^t; j) = \frac{\partial(-\ln(1 - h_j))}{\partial \theta} = -\frac{1}{1 - h_j} \cdot \frac{\partial(1 - h_j)}{\partial \theta} \quad (29)$$

$$= \frac{1}{1 - h_j} \cdot h_j(1 - h_j) \cdot \frac{\partial z_j}{\partial \theta} \quad (30)$$

$$= h_j \cdot \frac{\partial z_j}{\partial \theta} \quad (31)$$

$$h_w(\theta^t, w^t; j) = \frac{\partial(-\ln(1 - h_j))}{\partial w} = -\frac{1}{1 - h_j} \cdot \frac{\partial(1 - h_j)}{\partial w} \quad (32)$$

$$= \frac{1}{1 - h_j} \cdot h_j(1 - h_j) \cdot \frac{\partial z_j}{\partial w} \quad (33)$$

$$= h_j \cdot u_j \quad (34)$$

where $h_j = \frac{1}{1+e^{-z_j}}$ is the sigmoid output, $z_j = w^T u_j$ is the linear combination, and u_j are the filter outputs for sample j .

Combining both cases: For any sample j , we can write:

$$h_\theta(\theta^t, w^t; j) = (h_j - y_j) \cdot \frac{\partial z_j}{\partial \theta} \quad (35)$$

$$h_w(\theta^t, w^t; j) = (h_j - y_j) \cdot u_j \quad (36)$$